Test/git-issues/git-issue-2693.dfy
@@ -1,0 +1,51 @@
+// RUN: %exits-with 4 %dafny /compile:0 "%s" > "%t"
+// RUN: %diff "%s.expect" "%t"
+
+module A {
+  method Test() returns (result: Result)
+    ensures result.Bad? ==> result.c.IsFailure()
+  {
+    var c := new EvenGood_OddBad;
+    c.a := 0;
+    var x :- IncreaseAndReturn(c); // error: postcondition failure; deprecation warnings: PropagateFailure/Extract are methods
+    assert !c.IsFailure(); // error: assertion failure
+    return Good(x);
+  }
+
+  class EvenGood_OddBad {
+    var a: int
+
+    function method IsFailure(): bool
+      reads this
+    {
+      a % 2 == 1
+    }
+
+    method PropagateFailure() returns (r: Result)
+      requires IsFailure()
+      modifies this
+    {
+      a := 0;
+      return Bad(this);
+    }
+
+    method Extract() returns (x: int)
+      requires !IsFailure()
+      modifies this
+    {
+      x := a;
+      a := 19;
+    }
+  }
+
+  datatype Result = Good(x: int) | Bad(c: EvenGood_OddBad)
+
+  method IncreaseAndReturn(c: EvenGood_OddBad) returns (r: EvenGood_OddBad)
+    modifies c
+    ensures old(c.a) <= c.a && r == c
+  {
+    var n: nat;
+    c.a := c.a + n;
+    return c;
+  }
+}
