Test/git-issues/git-issue-817d.dfy
@@ -5,7 +5,7 @@ module M {
   datatype Result<T> = Failure(msg: string) | Success(value: T) {
     predicate method IsFailure() { Failure? }
     function method PropagateFailure(): Result<T> requires IsFailure() { this }
-    method Extract() returns (t: T) requires !IsFailure() ensures t == this.value { return this.value; }
+    function method Extract(): T requires !IsFailure() { this.value }
   }
 
   method mm() returns (rr: Result<int>) {
